Continued attempts to fix recursion inside isValidType, encountering issues since the only way to order the types is how deep the constructions go, but the only way to measure that is through recursion on TyCons

Constructions/epsilon.ml
@@ -3,7 +3,7 @@
 (*Defines type and term as is defined in John Harisson's paper
 TyBar -> String representing a type variable
 TyCons -> String representing a constructed type, followed by a type and a list of types.*) 
-define_type "type = 
+let lt, rt = define_type "type = 
 				    TyVar string
 			 	  | TyCons string ((type)list)";;    
 
@@ -94,9 +94,9 @@ let isValidConstName = define `
 (*Checks that a type is a valid type*)
 let isValidType = define `
 	(isValidType (TyVar str) = T) /\
-	(isValidType (TyCons str []) = EX (\x. x = str) ["epsilon";"type";"4";"3";"2";"int";"real";"hreal";"nadd";"char";"num";"ind";"1";"bool"]) /\
-	(isValidType (TyCons str [(a:type)]) = (EX (\x. x = str) ["finite_image";"list";"option";"recspace"])) /\
-	(isValidType (TyCons str [(a:type);(b:type)]) = (EX (\x. x = str) ["finite_prod";"finite_diff";"finite_sum";"cart";"sum";"prod";"fun"]))
+	(isValidType (TyCons str []) = (EX (\x. x = str) ["epsilon";"type";"4";"3";"2";"int";"real";"hreal";"nadd";"char";"num";"ind";"1";"bool"])) /\
+	(isValidType (TyCons str [a]) = ((isValidType a) /\ (EX (\x. x = str) ["finite_image";"list";"option";"recspace"]))) /\
+	(isValidType (TyCons str [(a:type);(b:type)]) = ((isValidType a) /\ (isValidType b) /\ (EX (\x. x = str) ["finite_prod";"finite_diff";"finite_sum";"cart";"sum";"prod";"fun"])))
 `;;
 
 (*This function will take a variable term, and another term of type epsilon, and return whether or not the types mismatch. If the term is not found, false is returned.
@@ -108,6 +108,70 @@ let typeMismatch = define `
 (typeMismatch (QuoVar name ty) (App e1 e2) = ((typeMismatch (QuoVar name ty) e1) \/ (typeMismatch (QuoVar name ty) e2))) /\
 (typeMismatch (QuoVar name ty) (Abs e1 e2) = ((typeMismatch (QuoVar name ty) e1) \/ (typeMismatch (QuoVar name ty) e2))) /\
 (typeMismatch (QuoVar name ty) (Quote e) = (typeMismatch (QuoVar name ty) e))`;;
+
+(*The below is temporary testing code while I try to get isValidType to recurse properly*)
+let rc = prove_general_recursive_function_exists `?rc.
+(rc [] = 0) /\
+(rc (CONS (TyVar str) t) = 1 + (rc t)) /\
+(rc (CONS (TyCons str l) t) = 1 + (rc l) + (rc t)) 
+`;;
+
+let test = define `
+	(lrt (a:type) (TyVar str) = F) /\
+	(lrt (a:type) (TyCons str []) = F) /\
+	(lrt (a:type) (TyCons str [b]) = (a=b)) /\
+	(lrt (a:type) (TyCons str [b;c]) = (a = b \/ a = c))
+`;;
+
+let SUM = new_recursive_definition list_RECURSION
+  `(SUM [] = 0) /\
+   (SUM (CONS h t) = h + SUM t)`;;
+
+let getList = define `
+	(getList (TyCons str lt)) = (lt)
+`;;
+
+let flattenlist = define `
+	(flattenlist (TyCons str lt) = 1 + (SUM (MAP flattenlist lt))) /\
+	(flattenlist (TyVar str) = 1)
+`;;
+
+
+let flatten = prove_general_recursive_function_exists `?flatten.
+	(flatten [] = 0) /\
+	(flatten [(TyCons str l)] = 1 + (flatten l)) /\
+	(flatten [(TyVar str)] = 1) /\
+	(flatten [(TyCons str l);(TyVar str2)] = 2 + (flatten l)) /\
+	(flatten [(TyVar str);(TyCons str2 l)] = 2 + (flatten l)) /\
+	(flatten [(TyVar str);(TyVar str2)] = 2) /\
+	(flatten [(TyCons str l);(TyCons str2 l2)] = 2 + (flatten l) + (flatten l2))
+`;;
+
+let so0 = prove_general_recursive_function_exists `?so0.
+	(so0 (TyVar str) = 1) /\
+	(so0 (TyCons str l) = (SUM (MAP so0 l)) + 1)
+`;;
+
+let so1 = define `
+	(so1 (a:type) (TyVar str) = F) /\
+	(so1 (a:type) (TyCons str l) = (EX (\x. x = a) l))
+`;;
+
+
+let isValidType = prove_general_recursive_function_exists `?isValidType.
+	(isValidType (TyVar str) = T) /\
+	(isValidType (TyCons str []) = (EX (\x. x = str) ["epsilon";"type";"4";"3";"2";"int";"real";"hreal";"nadd";"char";"num";"ind";"1";"bool"])) /\
+	(isValidType (TyCons str [a]) = ((isValidType a) /\ (EX (\x. x = str) ["finite_image";"list";"option";"recspace"]))) /\
+	(isValidType (TyCons str [(a:type);(b:type)]) = ((isValidType a) /\ (isValidType b) /\ (EX (\x. x = str) ["finite_prod";"finite_diff";"finite_sum";"cart";"sum";"prod";"fun"])))
+`;;
+
+let listUnordered = prove_general_recursive_function_exists `?luo.
+	luo [] = F /\
+	luo [a] = F /\
+	luo [b;c] = ((luo [c]) \/ (luo [b]))
+`;;
+
+(*End of testing code*)
 
 (*
 (*Mathematical definition of what constitutes a correct expression*)
